

$$(b \wedge a) \vee (b \wedge a) \vee (d \wedge (b \vee c))$$

①

1)

$$x_1 \Leftrightarrow b \wedge a$$

$$x_2 \Leftrightarrow \bar{x}_1$$

$$x_3 \Leftrightarrow b \vee c$$

$$x_4 \Leftrightarrow d \wedge x_3$$

$$x_5 \Leftrightarrow x_1 \vee x_2$$

$$x_6 \Leftrightarrow x_5 \vee x_4$$

$$(x_1 \vee a), (x_1 \vee b), (x_1 \vee \bar{a} \vee \bar{b})$$

$$(x_2 \vee x_1), (\bar{x}_2 \vee \bar{x}_1)$$

$$(x_3 \vee \bar{b}), (x_3 \vee \bar{c}), (\bar{x}_3 \vee b \vee c)$$

$$(x_4 \vee d), (x_4 \vee x_3), (x_4 \vee d \vee \bar{x}_3)$$

$$(x_5 \vee x_1), (x_5 \vee x_2), (x_5 \vee \bar{x}_1 \vee \bar{x}_2)$$

$$(x_6 \vee \bar{x}_5), (x_6 \vee \bar{x}_4), (\bar{x}_6 \vee x_5 \vee x_4)$$

2)

$$\Phi' = x_6 \wedge (x_5 \vee x_4 \rightarrow x_6) \wedge (x_5 \Leftrightarrow x_1 \vee x_2) \wedge (x_4 \Leftrightarrow d \wedge x_3) \wedge (x_3 \Leftrightarrow b \vee c) \wedge (x_2 \Leftrightarrow \bar{x}_1) \wedge (x_1 \Leftrightarrow b \wedge a)$$

3)

$$(a \wedge b) \vee (a \wedge \bar{b}) \vee (a \wedge (b \vee c))$$

②

$$X_1 \rightarrow (a \wedge b)$$

$$(\bar{x}_1 \vee a)(\bar{x}_1 \vee b)$$

$$\bar{x}_1 \rightarrow x_2$$

$$(x_1 \vee x_2)$$

$$x_3 \rightarrow (b \vee c)$$

$$(\bar{x}_3 \vee b \vee c)$$

$$x_4 \rightarrow (d \wedge x_3)$$

$$(\bar{x}_4 \vee d)(\bar{x}_4 \vee x_3)$$

$$x_5 \rightarrow (x_2 \vee x_1)$$

$$(\bar{x}_5 \vee x_2 \vee x_1)$$

$$x_6 \rightarrow (x_5 \vee x_4)$$

$$(\bar{x}_6 \vee x_5 \vee x_4)$$

2)

$$x_6 \wedge (x_6 \rightarrow x_5 \vee x_4) \wedge (x_5 \rightarrow x_2 \vee x_1) \wedge (x_4 \rightarrow (d \wedge x_3)) \wedge (x_3 \rightarrow (b \vee c)) \wedge (\bar{x}_1 \rightarrow x_2) \wedge (x_1 \rightarrow (a \wedge b))$$